ifc-machine/pico/tmu/cmach/Concrete.v
@@ -7,6 +7,7 @@ Require Import TMUInstr.
 Require Import CLattices.
 
 Set Implicit Arguments.
+Local Open Scope Z_scope.
 
 Section CMach.
 
@@ -18,19 +19,23 @@ Context {T: Type}
 Inductive CStkElmt := 
 | CData : @Atom T -> CStkElmt 
 | CRet : @Atom T -> bool -> bool -> CStkElmt.
+(* first bool is the type of call (v/void return), second bool is
+       saved privilege bit *)
 (* CH: not sure which variant is better, but in the Haskell version
        the first bool in CRet is labeled by the same label as the int *)
-(* second bool is saved privilege bit *)
 
+(* DD: the privileged parts of the states are now separate *)
 Record CS  := CState {
+  cache: list (@Atom T);
   mem : list (@Atom T);
+  fhdl:  list (@Instr T);
   imem : list (@Instr T);
   stk : list CStkElmt;
   pc : @Atom T;
   priv : bool
 }.
 
-Local Open Scope Z_scope.
+(** Running a whole piece of code contained in some interval of addresses *)
 Definition in_bounds (start_pc: Z) (end_pc: Z) (cs : CS) : Prop := 
   start_pc <= fst (pc cs) < end_pc. 
 
@@ -44,37 +49,8 @@ Proof.
     left; intuition; discriminate. 
 Qed. 
 
-(* [runsToEscape Rstep pc0 pc1 s0 s1] expresses that the machine runs without error
-from state s0 until the pc is no longer in the segment [pc0,pc1), at which 
-point it is state s1. *)
-Inductive runsToEscape (Rstep: CS -> CS -> Prop) (start_pc end_pc : Z): CS -> CS -> Prop :=
-| runsToEscapeDone : forall cs, 
-  ~ in_bounds start_pc end_pc cs -> 
-  runsToEscape Rstep start_pc end_pc cs cs
-| runsToEscapeStep: forall cs cs' cs'', 
-  in_bounds start_pc end_pc cs -> 
-  Rstep cs cs' -> 
-  runsToEscape Rstep start_pc end_pc cs' cs'' -> 
-  runsToEscape Rstep start_pc end_pc cs cs''.
-
-(* APT: I think the above definition is good enough to define handlerCorrect properly, below.
-But it is not constraining enough to prove the kind of composition property we'd like
-for composing adjacent fragments.  We want something like:
-
-Lemma runs_to_escape_compose: forall pc0 pc1 pc2 s0 s1 s2,
-  runsToEscape pc0 pc1 s0 s1 ->
-  fst (pc s1) = pc1 -> 
-  runsToEscape pc1 pc2 s1 s2 ->
-  runsToEscape pc0 pc2 s0 s2. 
-
-But this is false, because there might be jumps from one segment to the other.
-One way out of this is to strengthen runsToEscape so that code can only exit
-by (a) falling through; (b) jumping to the illegal address -1; or (c) returning
-to an address outside of the entire handler (e.g. >=  privInstSize).  If we then
-add hypothesis that [pc0,pc2) is within [0,privInstSize), this lemma should go through. *)
-
-(* Just for now, though, I'll define a more constrained version of the run predicate
-that requires code to reach end_pc. This should have the desired composition properties. *)
+(* More constrained version of the runToEscape predicate. Requires
+code to reach end_pc. This has the desired composition properties. *)
 Inductive runsToEnd (Rstep: CS -> CS -> Prop) (start_pc : Z) (end_pc : Z) : CS -> CS -> Prop :=
 | runsToEndDone : forall cs,
   start_pc <= end_pc -> (* this is technically useful *)
@@ -102,18 +78,6 @@ Proof.
       unfold in_bounds in *; omega. 
 Qed.
 
-(* A more generalized version that handles runsToEscape might also be useful. 
-   It might encode a rule like:
-
-   {P} E1 {Q;R}    {Q} E2 {S;R}
-----------------------------------
-       {P} E1; E2 {S;R}
-
-where {Q;R} means Q is the post-condition if code falls through
-and R is the post-condition if it jumps or returns to some other
-address outside of the privileged code segment. *)
-
-
 (* Self contained code: [runsToEnd' pc1 pc2 cs1 cs2] starts at pc2
 [pc1] and runs until pc [pc2]. *)
 Inductive runsToEnd' (Rstep: CS -> CS -> Prop) : Z -> Z -> CS -> CS -> Prop :=
@@ -134,28 +98,11 @@ Lemma runsToEnd'_compose : forall step pc0 pc1 s0 s1,
   runsToEnd' step pc1 pc2 s1 s2 ->
   runsToEnd' step pc0 pc2 s0 s2.
 Proof.
-  induction 1; intros.
-    auto.
-    econstructor; eauto.
+  induction 1; intros; eauto.
+  econstructor; eauto.
 Qed.
 
-(* TMU Stuff *)
-
-(* Where in the cache the various labels live *)
-Definition addrOpLabel  := 0.
-Definition addrTag1     := 1.
-Definition addrTag2     := 2.
-Definition addrTag3     := 3.
-Definition addrTagPC    := 4.
-Definition addrTagRes   := 5.
-Definition addrTagResPC := 6.
-
-Definition tmuCacheSize := 7.
-
-Definition privDataSize := tmuCacheSize. (* must be at least this big, but could
-                                              be bigger if fault handler wants private
-                                              storage. *)
-Definition privInstSize := 1000. (* arbitrary for now, but must be >= size of fault handler code *)
+Parameter runsToEscape : (CS -> CS -> Prop) -> Z -> Z -> CS -> CS -> Prop.
 
 (* Conversion between abstract labels (T) and tags (Z) *)
 Definition opCodeToZ (opcode : OpCode) : Z :=
@@ -173,11 +120,23 @@ match opcode with
 | OpVRet => 10
 end.
 
-(* TMU action on each instruction.  If rule is in the cache (currently
-just a single entry), leave the state unchanged and return
-Some(result_tag,result_pc_tag); otherwise, set the state to invoke the
-TMU fault handler code and return None. *)
+(* Where in the cache the various labels live *)
+Definition addrOpLabel  := 0.
+Definition addrTag1     := 1.
+Definition addrTag2     := 2.
+Definition addrTag3     := 3.
+Definition addrTagPC    := 4.
+Definition addrTagRes   := 5.
+Definition addrTagResPC := 6.
 
+Definition tmuCacheSize := 7.
+Definition privInstSize := 1000. 
+(* APT: arbitrary for now, but must be >= size of fault handler code 
+   DD: If we use this for specifying the complete execution of the fault handler, 
+   I suspect we want to give the exact size. *)
+  
+
+(** Cache spec when reading from, writing to *)
 Inductive tag_in_mem (m: list (@Atom T)) addr tagv : Prop := 
 | tim_intro : forall l, index_list_Z addr m = Some (tagv,l) ->
            tag_in_mem m addr tagv.
@@ -191,17 +150,13 @@ Inductive cache_hit (m: list (@Atom T)) : (Z * Z * Z * Z * Z ) -> Prop :=
                      (TAGPC: tag_in_mem m addrTagPC m_tagpc),
                 cache_hit m (m_op, m_tag1, m_tag2, m_tag3, m_tagpc).
 
-(* reads the cache line in non privileged mode, or ignore it in priv mode *)
+(* Reads the cache line in non privileged mode, or ignore it in priv mode *)
 Inductive cache_hit_read (m: list (@Atom T)) : bool -> T -> T -> Prop :=
 | chr_uppriv: forall m_tagr m_tagrpc,
               forall (TAG_Res: tag_in_mem m addrTagRes m_tagr)
                      (TAG_ResPC: tag_in_mem m addrTagResPC m_tagrpc),
                 cache_hit_read m false (ZToLab m_tagr) (ZToLab m_tagrpc)
 | chr_ppriv: cache_hit_read m true handlerLabel handlerLabel.
-
-Inductive check_addr_priv : bool -> Z -> Z -> Prop :=
-| cap_priv: forall addr size, check_addr_priv true addr size                              
-| cap_upriv: forall addr size, addr >= size -> check_addr_priv false addr size.
 
 Definition update_cache_spec_mvec (m m': list (@Atom T)) := 
   forall addr, 
@@ -215,6 +170,120 @@ Definition update_cache_spec_rvec (m m': list (@Atom T)) :=
   addr <> addrTagResPC -> 
   index_list_Z addr m = index_list_Z addr m'.
 
+(** Machine operations for popping the stack when executing a return instruction.
+    And it specs. *)
+
+Inductive c_pop_to_return : list CStkElmt -> list CStkElmt -> Prop := 
+| cptr_done: forall a b p s,
+   c_pop_to_return ((CRet a b p)::s) ((CRet a b p)::s)
+| cptr_pop: forall a s s',
+    c_pop_to_return s s' ->
+    c_pop_to_return ((CData a)::s) s'.
+
+Lemma c_pop_to_return_ret : forall s1 s2,
+  c_pop_to_return s1 s2 ->
+  exists a b p s, s2 = (CRet a b p)::s.
+Proof.
+  induction 1; intros; simpl; eauto.
+Qed.  
+  
+Lemma c_pop_to_return_spec : forall s1 s2,
+  c_pop_to_return s1 s2 ->
+  exists dstk, exists stk a b p,   
+    s1 = dstk++(CRet a b p)::stk
+    /\ (forall e, In e dstk -> exists a, e = CData a).
+Proof.
+  induction 1; intros; simpl in *. 
+  exists nil ; exists s ; exists a ; exists b ; exists p.
+  simpl ; split ; eauto.
+  intuition.
+
+  destruct IHc_pop_to_return as [dstk [stk [a0 [b0 [p0 [Hs Hdstk]]]]]].
+  subst.
+  exists ((CData a)::dstk).
+  exists stk ; eauto.
+  exists a0 ; exists b0 ; exists p0 ; split ; eauto.
+  intros. inv H0.
+  eauto.
+  eapply Hdstk; auto.
+Qed.
+
+Lemma c_pop_to_return_spec2: forall  s1 s2 p1 p2 b1 b2 a1 a2 dstk,
+ c_pop_to_return (dstk ++ CRet a1 b1 p1 :: s2) (CRet a2 b2 p2 :: s1) ->
+ (forall e, In e dstk -> exists a : @Atom T, e = CData a) ->
+ CRet a1 b1 p1 =  CRet a2 b2 p2.
+Proof.
+  induction dstk; intros.
+  inv H. auto.
+  simpl in *. 
+  inv H. destruct (H0 (CRet a2 b2 p2)). intuition. inv H.
+  eapply IHdstk; eauto.
+Qed.
+
+Lemma c_pop_to_return_spec3: forall s1 s2 b1 b2 p1 p2 a1 a2 dstk,
+ c_pop_to_return (dstk ++ CRet a1 b1 p1 :: s2) (CRet a2 b2 p2 :: s1) ->
+ (forall e, In e dstk -> exists a : @Atom T, e = CData a) ->
+ s1 = s2.
+Proof.
+  induction dstk; intros.
+  inv H. auto.
+  simpl in *. 
+  inv H. destruct (H0 (CRet a2 b2 p2)). intuition. inv H.
+  eapply IHdstk; eauto.
+Qed.
+
 End CMach.
 
-Hint Constructors cache_hit_read check_addr_priv.
+Notation read_m := index_list_Z.
+Notation upd_m := update_list_Z. 
+Notation "a ::: b" := ((CData a) :: b)  (at level 60, right associativity).
+Hint Constructors cache_hit cache_hit_read.
+
+
+(* DD: NOT NEEDED ANYMORE. TWO SEPARATE MODES and MEMORIES FOR THE MACHINE *)
+(* Inductive check_addr_priv : bool -> Z -> Z -> Prop := *)
+(* | cap_priv: forall addr size, check_addr_priv true addr size                    *)
+(* | cap_upriv: forall addr size, addr >= size -> check_addr_priv false addr size. *)
+
+
+(* DD: NOT VALID ANYMORE. KEEP IT FOR THE RECORD *)
+(* [runsToEscape Rstep pc0 pc1 s0 s1] expresses that the machine runs without error
+from state s0 until the pc is no longer in the segment [pc0,pc1), at which 
+point it is state s1. *)
+(* Inductive runsToEscape (Rstep: CS -> CS -> Prop) (start_pc end_pc : Z): CS -> CS -> Prop :=
+| runsToEscapeDone : forall cs, 
+  ~ in_bounds start_pc end_pc cs -> 
+  runsToEscape Rstep start_pc end_pc cs cs
+| runsToEscapeStep: forall cs cs' cs'', 
+  in_bounds start_pc end_pc cs -> 
+  Rstep cs cs' -> 
+  runsToEscape Rstep start_pc end_pc cs' cs'' -> 
+  runsToEscape Rstep start_pc end_pc cs cs''.*)
+
+(* APT: I think the above definition is good enough to define handlerCorrect properly, below.
+But it is not constraining enough to prove the kind of composition property we'd like
+for composing adjacent fragments.  We want something like:
+
+Lemma runs_to_escape_compose: forall pc0 pc1 pc2 s0 s1 s2,
+  runsToEscape pc0 pc1 s0 s1 ->
+  fst (pc s1) = pc1 -> 
+  runsToEscape pc1 pc2 s1 s2 ->
+  runsToEscape pc0 pc2 s0 s2. 
+
+But this is false, because there might be jumps from one segment to the other.
+One way out of this is to strengthen runsToEscape so that code can only exit
+by (a) falling through; (b) jumping to the illegal address -1; or (c) returning
+to an address outside of the entire handler (e.g. >=  privInstSize).  If we then
+add hypothesis that [pc0,pc2) is within [0,privInstSize), this lemma should go through. *)
+
+(* A more generalized version that handles runsToEscape might also be useful. 
+   It might encode a rule like:
+
+   {P} E1 {Q;R}    {Q} E2 {S;R}
+----------------------------------
+       {P} E1; E2 {S;R}
+
+where {Q;R} means Q is the post-condition if code falls through
+and R is the post-condition if it jumps or returns to some other
+address outside of the privileged code segment. *)
+
